Iris/IrisTest/HeapLang.lean
@@ -4,6 +4,8 @@ public import IrisTest.HeapLang.Linter
 public import IrisTest.HeapLang.Notation
 public import IrisTest.HeapLang.WeakestPre
 public import IrisTest.HeapLang.HeapTactics
+public import IrisTest.HeapLang.Apply
 public import IrisTest.HeapLang.Linter
 public import IrisTest.HeapLang.Par
+public import IrisTest.HeapLang.Semantics
 public import IrisTest.HeapLang.Tactics
